**3.2-1:**

> Show that if f(n) and g(n) are monotonically increasing functions, then so are the functions f(n) + g(n) and f(g(n)), and if f(n) and g(n) are in addition nonnegative, then f(n) * g(n) is monotonically increasing

Monotonically increasing functions essentially just means that if we have a function and two possible inputs `m` and `n` where `m <= n` then `f(m) <= f(n)`. If we were to substitue f(n) and g(n) with functions such as: f(n) = 2x and g(n) = x<sup>2</sup> these would be monotonically increasing nonnegative functions.

Therefore:

- f(n) + g(n) &equals; x<sup>2</sup> + 2x
- f(g(n)) &equals; 2(x<sup>2</sup>)
- f(n) * g(n) &equals; 2x<sup>3</sup>

In all of these cases, if we were to set the value of x to `m` instead of `n` where `m <= n`, the output with `m` would be less than or equal to that of `n`.

The more mathematical way of expressing this is:

f(n) + g(n):

```
f(m) <= f(n) for m <= n
g(m) <= g(n) for m <= n
f(m) + g(m) <= f(n) + g(n) for m <= n
```

f(g(n)):

```
f(g(m)) <= f(g(n)) for m <= n
```

This is true since g(m) <= g(n) since it is given that is monotonically increasing (as is f(n)).

f(n) * g(n):

```
f(m) * g(m) <= f(n) * g(n)
```
